added aes-gcm

code/experimental/aes/Hacl.Aes.NI.fst
@@ -31,6 +31,14 @@ val aes128_init: ctx:aes_ctx -> key:skey -> nonce:lbuffer uint8 12ul -> ST unit
 let aes128_init ctx key nonce = aes128_init #MAES ctx key nonce
 
 [@ CInline ]
+val aes128_set_nonce: ctx:aes_ctx -> nonce:lbuffer uint8 12ul -> ST unit
+			     (requires (fun h -> live h ctx /\ live h nonce))
+			     (ensures (fun h0 b h1 -> modifies (loc ctx) h0 h1))
+[@ CInline ]
+let aes128_set_nonce ctx nonce = aes128_set_nonce #MAES ctx nonce
+
+
+[@ CInline ]
 val aes128_key_block: kb:lbuffer uint8 16ul -> ctx:aes_ctx -> counter:size_t -> ST unit
 			     (requires (fun h -> live h kb /\ live h ctx))
 			     (ensures (fun h0 _ h1 -> modifies (loc kb) h0 h1))
@@ -39,17 +47,17 @@ let aes128_key_block kb ctx counter = aes128_key_block #MAES kb ctx counter
 
 
 inline_for_extraction
-val aes_update4: out:lbuffer uint8 64ul -> inp:lbuffer uint8 64ul -> ctx:aes_ctx -> counter:size_t -> rounds:size_t -> ST unit
+val aes128_update4: out:lbuffer uint8 64ul -> inp:lbuffer uint8 64ul -> ctx:aes_ctx -> counter:size_t -> ST unit
 			     (requires (fun h -> live h out /\ live h inp /\ live h ctx))
 			     (ensures (fun h0 b h1 -> modifies (loc out) h0 h1))
-let aes_update4 out inp ctx ctr rounds = aes_update4 #MAES out inp ctx ctr rounds
+let aes128_update4 out inp ctx ctr = aes_update4 #MAES out inp ctx ctr 10ul
 
 [@ CInline ]
-val aes_ctr: len:size_t -> out:lbuffer uint8 len -> inp:lbuffer uint8 len -> ctx:aes_ctx -> counter:size_t -> rounds:size_t -> ST unit
+val aes128_ctr: len:size_t -> out:lbuffer uint8 len -> inp:lbuffer uint8 len -> ctx:aes_ctx -> counter:size_t -> ST unit
 			     (requires (fun h -> live h out /\ live h inp /\ live h ctx))
 			     (ensures (fun h0 _ h1 -> modifies (loc out) h0 h1))
 [@ CInline ]
-let aes_ctr len out inp ctx counter rounds = aes_ctr #MAES len out inp ctx counter rounds
+let aes128_ctr len out inp ctx counter  = aes_ctr #MAES len out inp ctx counter 10ul
 
 [@ CInline ]
 let aes128_ctr_encrypt len out inp k n c = aes128_ctr_encrypt #MAES len out inp k n c
