code/experimental/gf128/Hacl.Gf128.NI.fst
@@ -21,21 +21,19 @@ val gcm_init: ctx:gcm_ctx -> key:lbuffer uint8 16ul -> Stack unit
 let gcm_init ctx key = gcm_init #FNI ctx key
 
 
-val gcm_update_blocks4: ctx:gcm_ctx -> len:size_t{v len % 64 == 0} -> text:lbuffer uint8 len -> Stack unit
-	  (requires (fun h -> live h ctx /\ live h text))
-	  (ensures (fun h0 _ h1 -> modifies (loc ctx) h0 h1))
-let gcm_update_blocks4  ctx len text = poly4_add_mul #FNI ctx len text
-
+[@ CInline ]
 val gcm_update_blocks: ctx:gcm_ctx -> len:size_t{v len % 16 == 0} -> text:lbuffer uint8 len -> Stack unit
 	  (requires (fun h -> live h ctx /\ live h text))
 	  (ensures (fun h0 _ h1 -> modifies (loc ctx) h0 h1))
-let gcm_update_blocks  ctx len text = poly #FNI ctx len text
+let gcm_update_blocks  ctx len text = poly4_add_mul #FNI ctx len text
 
-val gcm_update_last: ctx:gcm_ctx -> len:size_t{v len < 16} -> text:lbuffer uint8 len -> Stack unit
+[@ CInline ]
+val gcm_update_padded: ctx:gcm_ctx -> len:size_t -> text:lbuffer uint8 len -> Stack unit
 	  (requires (fun h -> live h ctx /\ live h text))
 	  (ensures (fun h0 _ h1 -> modifies (loc ctx) h0 h1))
-let gcm_update_last  ctx len text = poly #FNI ctx len text
+let gcm_update_padded  ctx len text = poly4_add_mul #FNI ctx len text
 
+[@ CInline ]
 val gcm_emit: tag:lbuffer uint8 16ul -> ctx:gcm_ctx  -> Stack unit
 	  (requires (fun h -> live h ctx /\ live h tag))
 	  (ensures (fun h0 _ h1 -> modifies (loc tag) h0 h1))
@@ -43,6 +41,7 @@ let gcm_emit tag ctx =
     let acc = get_acc ctx in
     decode tag acc
 
+[@ CInline ]
 val ghash: tag:block -> len:size_t -> text:lbuffer uint8 len -> key:block -> Stack unit
 	  (requires (fun h -> live h tag /\ live h text /\ live h key))
 	  (ensures (fun h0 _ h1 -> modifies (loc tag) h0 h1))
